message_eq changes

KeyManagement/Simulation.v
@@ -7,12 +7,13 @@ From Coq Require Import
 
 Require Import
         MyPrelude
+        (* AdversaryUniverse *)
         Maps
+        MessageEq
         Common
         MapLtac
         Keys
-        Tactics
-        Messages.
+        Tactics.
 
 Require IdealWorld
         RealWorld.
@@ -26,10 +27,10 @@ Hint Resolve in_eq in_cons.
 Remove Hints absurd_eq_true trans_eq_bool.
 
 Definition rstepSilent {A B : Type} (U1 U2 : RealWorld.universe A B) :=
-  RealWorld.step_universe U1 Silent U2.
+  RealWorld.step_universe U1 Messages.Silent U2.
 
 Definition istepSilent {A : Type} (U1 U2 : IdealWorld.universe A) :=
-  IdealWorld.lstep_universe U1 Silent U2.
+  IdealWorld.lstep_universe U1 Messages.Silent U2.
 
 Inductive chan_key : Set :=
 | Public (ch_id : IdealWorld.channel_id)
@@ -42,159 +43,62 @@ Inductive chan_key : Set :=
     -> k2.(keyUsage) = Encryption
     -> chan_key
 .
-Definition message_matches (n : nat) := if n then True else False.
-  
-Inductive action_matches {A B} :
-    RealWorld.action * RealWorld.universe A B -> IdealWorld.action * IdealWorld.universe A -> Prop :=
-| Inp : forall t__r t__i (msg1 : RealWorld.message t__r) (msg2 : IdealWorld.message t__i) a__rw a__iw ch_id cs ps p y U__iw U__rw,
-      a__rw = (RealWorld.Input msg1 p y)
-    -> a__iw = IdealWorld.Input msg2 ch_id cs ps
-    -> MessageEq.message_matches  (msg1, U__rw) (msg2, U__iw)
-    -> action_matches (a__rw, U__rw)
-                     (a__iw, U__iw)
-| Out : forall t__r t__i (msg1 : RealWorld.message t__r) (msg2 : IdealWorld.message t__i) a__rw a__iw ch_id cs ps U__iw U__rw,
-      a__rw = RealWorld.Output msg1
-    -> a__iw = IdealWorld.Output msg2 ch_id cs ps
-    -> MessageEq.message_matches (msg1, U__rw) (msg2, U__iw)
-    -> action_matches (a__rw, U__rw)
-                     (a__iw, U__iw)
+
+(* Inductive msg_eq : forall t__r t__i, *)
+(*     RealWorld.crypto t__r *)
+(*     -> IdealWorld.message.message t__i * IdealWorld.channel_id * IdealWorld.channels * IdealWorld.permissions -> Prop := *)
+
+(* (* Still need to reason over visibility of channel -- plaintext really means everyone can see it *) *)
+(* | PlaintextMessage' : forall content ch_id cs ps, *)
+(*     ps $? ch_id = Some (IdealWorld.construct_permission true true) -> *)
+(*     msg_eq (RealWorld.Content content) (IdealWorld.message.Content content, ch_id, cs, ps) *)
+(* . *)
+
+Inductive action_matches :
+    RealWorld.action -> IdealWorld.action -> Prop :=
+| Inp : forall t__r t__i (msg1 : RealWorld.crypto t__r) (msg2 : IdealWorld.message.message t__i) rw iw ch_id cs ps p y,
+      rw = (RealWorld.Input msg1 p y)
+    -> iw = IdealWorld.Input msg2 ch_id cs ps
+    (* -> MessageEq.message_eq msg1 msg2 ch_id cs ps *)
+    -> action_matches rw iw
+| Out : forall t__r t__i (msg1 : RealWorld.crypto t__r) (msg2 : IdealWorld.message.message t__i) rw iw ch_id cs ps,
+      rw = RealWorld.Output msg1
+    -> iw = IdealWorld.Output msg2 ch_id cs ps
+    (* -> msg_eq msg1 (msg2, ch_id, cs, ps) *)
+    -> action_matches rw iw
 .
 
 Section RealWorldUniverseProperties.
   Import RealWorld.
 
-Section RealWorldUniverseProperties.
-  Import RealWorld.
-
-  Definition testHygProto1 := Gen.
-
-  Lemma testHygProto1_ok :
-    protocol_hygienic [] testHygProto1.
-||||||| merged common ancestors
-  (*       -> cs' = match msg with *)
-  (*               | Plaintext _ => cs' *)
-  (*               | KeyMessage _ => cs' *)
-  (*               | MsgPair m1 m2 => cs' *)
-  (*               | SignedCiphertext _ _ c_id => c_id :: cs *)
-  (*               | Signature m _ c_id => c_id :: cs *)
-  (*               end *)
-  Definition ciphers_of {t} (msg : message t) : list cipher_id :=
-    match msg with
-    | SignedCiphertext _ _ c_id => [c_id]
-    | Signature _ _ c_id        => [c_id]
-    | _                         => []
-    end.
-
-  (* Fixpoint build_expr_value {A} (cmd : user_cmd A) : A := *)
-  (*   match cmd with *)
-  (*   | Return a => a *)
-  (*   | Bind cmd1 cmd2 => build_expr_value (cmd2 (build_expr_value cmd1)) *)
-  (*   | Gen => 1 *)
-  (*   | Send _ _ => tt *)
-  (*   | Recv _ => forall {t} (msg : message t), msg *)
-  (*   | SignEncrypt _ _ _ => forall msg, msg *)
-  (*   | Decrypt _ => forall msg, msg *)
-  (*   | Sign _ _ => forall msg, msg *)
-  (*   | Verify _ _ => true *)
-  (*   | GenerateSymKey  _ => (1,true) *)
-  (*   | GenerateAsymKey  _ => (1,true) *)
-  (*   end. *)
-
-  (* Fixpoint build_def_value {A} (cmd : user_cmd A) : option A := *)
-  (*   match cmd with *)
-  (*   | Return a => Some a *)
-  (*   | Bind cmd1 cmd2 => build_expr_value (cmd2 (build_expr_value cmd1)) *)
-  (*   | Gen => Some 1 *)
-  (*   | Send _ _ => Some tt *)
-  (*   | Recv _ => forall {t} (msg : message t), msg *)
-  (*   | SignEncrypt _ _ _ => forall msg, msg *)
-  (*   | Decrypt _ => forall msg, msg *)
-  (*   | Sign _ _ => forall msg, msg *)
-  (*   | Verify _ _ => Some true *)
-  (*   | GenerateSymKey  _ => Some (1,true) *)
-  (*   | GenerateAsymKey  _ => Some (1,true) *)
-  (*   end. *)
-
-  Inductive protocol_hygienic (cs : list cipher_id): forall {A}, user_cmd A -> Prop :=
-  | BindRecvHygienic :
-      forall {A t} (rec : user_cmd (message t)) (cmd : message t -> user_cmd A) pat,
-        rec = Recv pat
-        -> (forall cs' msg,
-              cs' = ciphers_of msg ++ cs
-              -> protocol_hygienic cs' (cmd msg)
-          )
-        -> protocol_hygienic cs (Bind rec cmd)
-  | BindHygienic : forall {A B} (rec : user_cmd B) (cmd : B -> user_cmd A) b,
-        protocol_hygienic cs (cmd b)
-        -> protocol_hygienic cs (Bind rec cmd)
-  | ReturnHygienic : forall {A} (a : A),
-      protocol_hygienic cs (Return a)
-  | GenHygienic :
-      protocol_hygienic cs Gen
-  | SendHygienic : forall {t} (uid : user_id) (msg : message t),
-      protocol_hygienic cs (Send uid msg)
-  | RecvHygienic : forall {t} pat,
-      protocol_hygienic cs (@Recv t pat)
-  | SignEncryptHygienic : forall {t} (msg : message t) k__s k__e,
-      protocol_hygienic cs (SignEncrypt k__s k__e msg)
-  | DecryptHygienic : forall {t} msg k__s k__e c_id,
-      msg = SignedCiphertext k__s k__e c_id
-      -> List.In c_id cs
-      -> protocol_hygienic cs (@Decrypt t msg)
-  | SignHygienic : forall {t} (msg : message t) k,
-      protocol_hygienic cs (Sign k msg)
-  | VerifyHygienic : forall {t} msg msg' k kp c_id,
-      msg = Signature msg' k c_id
-      -> List.In c_id cs
-      -> protocol_hygienic cs (@Verify t kp msg).
-
-  (* Inductive protocol_hygienic' (cs__in cs__out : list cipher_id): forall {A}, user_cmd A -> Prop := *)
-  (* | BindHygienic' : *)
-  (*     forall {B} (cmd : user_cmd B) (proc : B -> user_cmd A), *)
-  (*       protocol_hygienic' cs__in cmd cs__out *)
-  (*       -> protocol_hygienic' cs__out proc cs__in *)
-  (* | ReturnHygienic' : forall {A} (a : A), *)
-  (*     protocol_hygienic cs (Return a) cs *)
-  (* | GenHygienic' : *)
-  (*     protocol_hygienic' cs Gen cs *)
-  (* | SendHygienic' : forall {t} (uid : user_id) (msg : message t), *)
-  (*     protocol_hygienic' cs (Send uid msg) cs *)
-  (* | RecvHygienic' : forall {t} pat, *)
-  (*     protocol_hygienic cs (@Recv t pat) *)
-
-  (* | SignEncryptHygienic : forall {t} (msg : message t) k__s k__e, *)
-  (*     protocol_hygienic cs (SignEncrypt k__s k__e msg) *)
-  (* | DecryptHygienic : forall {t} msg k__s k__e c_id, *)
-  (*     msg = SignedCiphertext k__s k__e c_id *)
-  (*     -> List.In c_id cs *)
-  (*     -> protocol_hygienic cs (@Decrypt t msg) *)
-  (* | SignHygienic : forall {t} (msg : message t) k, *)
-  (*     protocol_hygienic cs (Sign k msg) *)
-  (* | VerifyHygienic : forall {t} msg msg' k kp c_id, *)
-  (*     msg = Signature msg' k c_id *)
-  (*     -> List.In c_id cs *)
-  (*     -> protocol_hygienic cs (@Verify t kp msg). *)
-
-
-
-  Definition user_protocols_hygienic {A B} (U : universe A B) :=
-    Forall_natmap (fun u => protocol_hygienic [] u.(protocol)) U.(users).
-
-  Hint Constructors protocol_hygienic.
-  Hint Extern 1 nat => exact 1.
-  Hint Extern 1 key_identifier => exact 1.
-
-  Definition testHygProto1 := Gen.
-
-  Lemma testHygProto1_ok :
-    protocol_hygienic [] testHygProto1.
-=======
   Variable honestk : key_perms.
 
+  (* Syntactic Predicates *)
   Definition keys_good (ks : keys) : Prop :=
     forall k_id k,
         ks $? k_id = Some k
       -> keyId k = k_id.
+
+  Definition msgCiphers_ok {t} (cs : ciphers) (msg : crypto t) :=
+    Forall (fun sigm => match sigm with
+                     | (existT _ _ m) =>
+                       match m with
+                       | SignedCiphertext k__sign k__enc msg_id
+                         => exists t (m' : crypto t), cs $? msg_id = Some (SigEncCipher k__sign k__enc m')
+                       | Signature m' k sig
+                         => cs $? sig = Some (SigCipher k m')
+                       | _ => False
+                       end
+                     end) (findMsgCiphers msg).
+
+  Definition ciphers_good (cs : ciphers) : Prop :=
+    Forall_natmap (fun c =>
+                     match c with
+                     | SigEncCipher k__sign k__enc m => msgCiphers_ok cs m
+                     | SigCipher k m => msgCiphers_ok cs m
+                     | _ => False
+                     end
+                  ) cs.
 
   Definition user_cipher_queue_ok (cs : ciphers) (honestk : key_perms) :=
     Forall (fun cid => exists c, cs $? cid = Some c
@@ -204,54 +108,29 @@ Section RealWorldUniverseProperties.
     Forall_natmap
       (fun u => user_cipher_queue_ok cs honestk u.(c_heap)) usrs.
 
-  Lemma cons_app_split :
-    forall {A} (l l1 l2 : list A) a,
-      a :: l = l1 ++ l2
-      -> (l1 = [] /\ l2 = a :: l)
-      \/ (exists l1', l1 = a :: l1' /\ l = l1' ++ l2).
->>>>>>> message_type_refactor
-  Proof.
-    destruct l1; eauto; intros.
-
-    right. invert H.
-    eexists; eauto.
-  Qed.
-
-  Definition msgCiphersSigned {t} (msg : message t) :=
-    (* Forall (fun m => let m := (existT _ _ msg) in msg_honestly_signed honestk msg = true) (findMsgCiphers msg). *)
-    Forall (fun sigm => match sigm with
-                     | (existT _ _ m) => msg_honestly_signed honestk m = true
-                     end) (findMsgCiphers msg).
-
-  Inductive encrypted_cipher_ok : cipher -> Prop :=
-  | SigCipherHonestOk : forall {t} (msg : message t) k,
+  Inductive encrypted_cipher_ok (cs : ciphers) : cipher -> Prop :=
+  | SigCipherHonestOk : forall {t} (msg : crypto t) k,
       honestk $? k = Some true
       -> (forall k, findKeys msg $? k = Some true -> False)
-      -> msgCiphersSigned msg
-      -> encrypted_cipher_ok (SigCipher k msg)
+      -> msgCiphersSigned honestk cs msg
+      -> encrypted_cipher_ok cs (SigCipher k msg)
   | SigCipherNotHonestOk : forall {t} (msg : message t) k,
       honestk $? k <> Some true
-      -> encrypted_cipher_ok (SigCipher k msg)
+      -> encrypted_cipher_ok cs (SigCipher k msg)
   | SigEncCipherAdvSignedOk :  forall {t} (msg : message t) k__e k__s,
       honestk $? k__s <> Some true
       -> (forall k, findKeys msg $? k = Some true
               -> honestk $? k <> Some true)
-      -> encrypted_cipher_ok (SigEncCipher k__s k__e msg)
-  (* | SigEncCipherHonestSignedEncKeyNotHonestOk : forall {t} (msg : message t) k__e k__s, *)
-  (*     honestk $? k__s = Some true *)
-  (*     -> honestk $? k__e <> Some true *)
-  (*     -> (forall k, findKeys msg $? k = Some true *)
-  (*             -> honestk $? k <> Some true) *)
-  (*     -> encrypted_cipher_ok (SigEncCipher k__s k__e msg) *)
+      -> encrypted_cipher_ok cs (SigEncCipher k__s k__e msg)
   | SigEncCipherHonestSignedEncKeyHonestOk : forall {t} (msg : message t) k__e k__s,
       honestk $? k__s = Some true
       -> honestk $? k__e = Some true
       -> keys_mine honestk (findKeys msg)
-      -> msgCiphersSigned msg
-      -> encrypted_cipher_ok (SigEncCipher k__s k__e msg).
+      -> msgCiphersSigned honestk cs msg
+      -> encrypted_cipher_ok cs (SigEncCipher k__s k__e msg).
 
-  Definition encrypted_ciphers_ok :=
-    Forall_natmap encrypted_cipher_ok.
+  Definition encrypted_ciphers_ok (cs : ciphers) :=
+    Forall_natmap (encrypted_cipher_ok cs) cs.
 
   Definition message_no_adv_private {t} (msg : message t) :=
     forall k, findKeys msg $? k = Some true -> False.
@@ -259,17 +138,24 @@ Section RealWorldUniverseProperties.
 
   Hint Unfold message_no_adv_private.
 
-  Definition message_queue_ok (msgs : queued_messages) :=
+  Definition adv_message_queue_ok (honestk : key_perms) (msgs : queued_messages) :=
+    Forall (fun sigm => match sigm with
+                     | (existT _ _ m) =>
+                       forall k, findKeys m $? k = Some true -> honestk $? k <> Some true
+                     end
+           ) msgs.
+
+  Definition message_queue_ok (cs : ciphers) (msgs : queued_messages) :=
     Forall (fun sigm => match sigm with
                      | (existT _ _ m) =>
                          msg_honestly_signed honestk m = true
                        -> message_no_adv_private m
-                       /\ msgCiphersSigned m
+                       /\ msgCiphersSigned honestk cs m
                      end
            ) msgs.
 
-  Definition message_queues_ok {A} (usrs : honest_users A) :=
-    Forall_natmap (fun u => message_queue_ok u.(msg_heap)) usrs.
+  Definition message_queues_ok {A} (cs : ciphers) (usrs : honest_users A) :=
+    Forall_natmap (fun u => message_queue_ok cs u.(msg_heap)) usrs.
 
   Definition adv_no_honest_keys (advk : key_perms) : Prop :=
     forall k_id,
@@ -277,10 +163,6 @@ Section RealWorldUniverseProperties.
       \/  honestk $? k_id = Some false
       \/ (honestk $? k_id = Some true /\ advk $? k_id <> Some true)
       ).
-
-  Definition is_powerless {B} (usr : user_data B) (b: B): Prop :=
-    adv_no_honest_keys usr.(key_heap)
-  /\ usr.(protocol) = Return b.
 
   Lemma adv_no_honest_keys_empty :
     adv_no_honest_keys $0.
@@ -302,59 +184,180 @@ Definition adv_universe_ok {A B} (U : RealWorld.universe A B) : Prop :=
   let honestk := RealWorld.findUserKeys U.(RealWorld.users)
   in  keys_good U.(RealWorld.all_keys)
     /\ user_cipher_queues_ok U.(RealWorld.all_ciphers) honestk U.(RealWorld.users)
-    /\ message_queues_ok honestk U.(RealWorld.users)
+    /\ message_queues_ok honestk U.(RealWorld.all_ciphers) U.(RealWorld.users)
+    /\ adv_message_queue_ok honestk U.(RealWorld.adversary).(RealWorld.msg_heap)
     /\ adv_no_honest_keys honestk U.(RealWorld.adversary).(RealWorld.key_heap).
 
-Definition simulates_silent_step {A B} (R : RealWorld.universe A B -> IdealWorld.universe A -> Prop) :=
-  forall U__r U__i,
-    R U__r U__i
+Section Simulation.
+  Variable A B : Type.
+  Variable advP : RealWorld.user_data B -> Prop.
+  Variable R : RealWorld.simpl_universe A -> IdealWorld.universe A -> Prop.
+
+  Definition simulates_silent_step :=
+    forall (U__r : RealWorld.universe A B) U__i,
+      R (RealWorld.peel_adv U__r) U__i
     -> universe_ok U__r
+    -> adv_universe_ok U__r
+    -> advP U__r.(RealWorld.adversary)
     -> forall U__r',
         rstepSilent U__r U__r'
         -> exists U__i',
-            istepSilent ^* U__i U__i'
-          /\ universe_ok U__r'
-          /\ R U__r' U__i'.
+          istepSilent ^* U__i U__i'
+        /\ R (RealWorld.peel_adv U__r') U__i'.
 
-Definition simulates_labeled_step {A B} (R : RealWorld.universe A B -> IdealWorld.universe A -> Prop) :=
-  forall U__r U__i,
-    R U__r U__i
+  Definition simulates_labeled_step :=
+    forall (U__r : RealWorld.universe A B) U__i,
+      R (RealWorld.peel_adv U__r) U__i
     -> universe_ok U__r
+    -> adv_universe_ok U__r
+    -> advP U__r.(RealWorld.adversary)
     -> forall a1 U__r',
         RealWorld.step_universe U__r (Action a1) U__r' (* excludes adversary steps *)
         -> exists a2 U__i' U__i'',
           istepSilent^* U__i U__i'
-          /\ IdealWorld.lstep_universe U__i' (Action a2) U__i''
-          /\ action_matches (a1, U__r) (a2, U__i)
-          /\ R U__r' U__i''
-          /\ universe_ok U__r'.
+        /\ IdealWorld.lstep_universe U__i' (Action a2) U__i''
+        /\ action_matches a1 a2
+        /\ R (RealWorld.peel_adv U__r') U__i''.
 
-Definition simulates_labeled_step_safe {A B} (R : RealWorld.universe A B -> IdealWorld.universe A -> Prop) :=
-  forall U__r U__i,
-    R U__r U__i
-    -> forall a (U U__r' : RealWorld.universe A B),
-      RealWorld.step_universe U (Action a) U__r' (* excludes adversary steps *)
-      -> RealWorld.findUserKeys U.(RealWorld.users) = RealWorld.findUserKeys U__r.(RealWorld.users)
-      ->  RealWorld.action_adversary_safe
-           (RealWorld.findUserKeys U__r.(RealWorld.users))
-           a.
+  Definition simulates_universe_ok :=
+    forall B (U__r : RealWorld.universe A B) U__i,
+        R (strip_adversary U__r) U__i
+      -> universe_ok U__r
+      -> adv_universe_ok U__r
+      -> forall U__r' lbl,
+        RealWorld.step_universe U__r lbl U__r'
+        -> universe_ok U__r'.
 
+  Definition simulates_labeled_step_safe :=
+    forall B (U__r : RealWorld.universe A B) U__i,
+      R (strip_adversary U__r) U__i
+      -> forall U__r' a,
+        RealWorld.step_universe U__r (Action a) U__r' (* excludes adversary steps *)
+        -> RealWorld.action_adversary_safe
+            (RealWorld.findUserKeys U__r.(RealWorld.users))
+            U__r.(RealWorld.all_ciphers)
+            a.
 
-Definition simulates {A B : Type}
-           (R : RealWorld.universe A B -> IdealWorld.universe A -> Prop)
-           (U__r : RealWorld.universe A B) (U__i : IdealWorld.universe A) :=
+  Definition simulates (U__r : RealWorld.universe A B) (U__i : IdealWorld.universe A) :=
 
-  (* conditions for simulation steps *)
-  simulates_silent_step R
-/\ simulates_labeled_step R
-/\ simulates_labeled_step_safe R
+    (* conditions for simulation steps *)
+    simulates_silent_step
+  /\ simulates_labeled_step
+  /\ simulates_universe_ok
+  /\ simulates_labeled_step_safe
 
   (* conditions for start *)
-/\ R U__r U__i
-/\ universe_ok U__r
-.
+  /\ R (RealWorld.peel_adv U__r) U__i
+  /\ universe_ok U__r
+  /\ adv_universe_ok U__r.
 
-Definition refines {A B : Type} (U1 : RealWorld.universe A B)(U2 : IdealWorld.universe A) :=
-  exists R, simulates R U1 U2.
+End Simulation.
 
-Infix "<|" := refines (no associativity, at level 70).
+Definition refines {A B : Type} (advP : RealWorld.user_data B -> Prop) (U1 : RealWorld.universe A B) (U2 : IdealWorld.universe A) :=
+  exists R, simulates advP R U1 U2.
+
+Notation "u1 <| u2 \ p " := (refines p u1 u2) (no associativity, at level 70).
+
+Definition lameAdv {B} (b : B) :=
+  fun adv => adv.(RealWorld.protocol) = RealWorld.Return b.
+
+Definition awesomeAdv : forall B, RealWorld.user_data B -> Prop :=
+  fun _ _ => True.
+
+
+Section RealWorldLemmas.
+
+  Import RealWorld.
+
+  Lemma msgCiphersSigned_addnl_cipher :
+    forall cs msgs honestk c_id c,
+      Forall (RealWorld.msgCipherOk honestk cs) msgs
+      -> ~ In c_id cs
+      -> Forall (RealWorld.msgCipherOk honestk (cs $+ (c_id,c))) msgs.
+  Proof.
+    induction msgs; intros; econstructor; invert H; eauto; clean_map_lookups.
+    unfold RealWorld.msgCipherOk in H3. unfold RealWorld.msgCipherOk.
+    destruct a; intuition idtac.
+    destruct m; eauto.
+    - invert H1; invert H2; repeat eexists.
+      destruct (c_id ==n msg_id); subst; clean_map_lookups; eauto.
+    - destruct (c_id ==n sig); subst; clean_map_lookups; eauto.
+  Qed.
+
+  Lemma encrypted_cipher_ok_addnl_cipher :
+    forall honestk cs c_id c1 c2,
+      encrypted_cipher_ok honestk cs c1
+      -> ~ In c_id cs
+      -> encrypted_cipher_ok honestk (cs $+ (c_id,c2)) c1.
+  Proof.
+    inversion 1; intros; try solve [ econstructor; eauto ].
+    - econstructor; eauto.
+      eapply msgCiphersSigned_addnl_cipher; auto.
+    - eapply SigEncCipherHonestSignedEncKeyHonestOk; eauto.
+      eapply msgCiphersSigned_addnl_cipher; auto.
+  Qed.
+
+  Lemma encrypted_ciphers_ok_addnl_cipher :
+    forall honestk cs c_id c,
+      Forall_natmap (encrypted_cipher_ok honestk cs) cs
+      -> ~ In c_id cs
+      -> Forall_natmap (encrypted_cipher_ok honestk (cs $+ (c_id, c))) cs.
+  Proof.
+    intros.
+    rewrite Forall_natmap_forall in *.
+    intros.
+    specialize (H _ _ H1); eauto using encrypted_cipher_ok_addnl_cipher.
+  Qed.
+
+  Hint Resolve
+       encrypted_ciphers_ok_addnl_cipher.
+
+  Lemma adv_step_encrypted_ciphers_ok :
+    forall {A B C} cs cs' lbl (usrs usrs' : honest_users A) (adv adv' : user_data B)
+              gks gks' ks ks' qmsgs qmsgs' mycs mycs' bd bd',
+      step_user lbl None bd bd'
+      -> forall (cmd : user_cmd C) honestk,
+        bd = (usrs, adv, cs, gks, ks, qmsgs, mycs, cmd)
+        -> honestk = findUserKeys usrs
+        -> ks = adv.(key_heap)
+        -> adv_no_honest_keys honestk ks
+        -> encrypted_ciphers_ok honestk cs
+        -> forall cmd' honestk',
+            bd' = (usrs', adv', cs', gks', ks', qmsgs', mycs', cmd')
+            -> honestk' = findUserKeys usrs'
+            -> encrypted_ciphers_ok honestk' cs'.
+  Proof.
+    induction 1; inversion 1; inversion 5; intros; subst;
+      eauto 2; autorewrite with find_user_keys; eauto.
+
+    - econstructor; eauto.
+      assert (adv_no_honest_keys (findUserKeys usrs') (key_heap adv')) as ADV by assumption.
+      specialize (H20 k__signid).
+      econstructor; eauto.
+      + unfold not; intros; split_ors; split_ands; contra_map_lookup; contradiction.
+      + intros.
+        specialize (H4 _ _ H6).
+        specialize (ADV k); unfold not; intros; split_ors; split_ands; contra_map_lookup; contradiction.
+
+    - econstructor; eauto.
+      specialize (H16 k_id).
+      eapply SigCipherNotHonestOk; unfold not; intros; split_ors; split_ands; contra_map_lookup; contradiction.
+  Qed.
+
+  Lemma universe_ok_adv_step :
+    forall {A B} (U__r : universe A B) lbl usrs adv cs gks ks qmsgs mycs cmd,
+      universe_ok U__r
+      -> adv_universe_ok U__r
+      -> step_user lbl None
+                  (users U__r, adversary U__r, all_ciphers U__r, all_keys U__r,
+                   key_heap (adversary U__r), msg_heap (adversary U__r),
+                   c_heap (adversary U__r), protocol (adversary U__r)) (usrs, adv, cs, gks, ks, qmsgs, mycs, cmd)
+      -> universe_ok
+          (buildUniverseAdv
+             usrs cs gks
+             {| key_heap := ks; protocol := cmd; msg_heap := qmsgs; c_heap := mycs |}).
+  Proof.
+    unfold universe_ok, adv_universe_ok; destruct U__r; simpl; intros; split_ands; eauto using adv_step_encrypted_ciphers_ok.
+  Qed.
+
+End RealWorldLemmas.
